utp/utp_tactics.thy
@@ -12,7 +12,7 @@ section {* UTP Tactics *}
 
 theory utp_tactics
   imports 
-    utp_expr utp_unrest utp_usedby
+    utp_expr utp_unrest
 keywords "update_uexpr_rep_eq_thms" :: thy_decl
 begin
 
@@ -156,7 +156,6 @@ declare uexpr_eq_iff [uexpr_transfer_laws]
 named_theorems uexpr_transfer_extra "extra simplifications for uexpr transfer"
   
 declare unrest_uexpr.rep_eq [uexpr_transfer_extra]
-  usedBy_uexpr.rep_eq [uexpr_transfer_extra]
   utp_expr.numeral_uexpr_rep_eq [uexpr_transfer_extra]
   utp_expr.less_eq_uexpr.rep_eq [uexpr_transfer_extra]
   Abs_uexpr_inverse [simplified, uexpr_transfer_extra]
